src/crypto_foundations/oracle_comp.lean
@@ -48,26 +48,124 @@ def decidable_eq_of_oracle_comp (oc : oracle_comp A B C) :
     (hoc (λ a, (oracle_comp_base_exists (ob s a) t).1) 
       (λ a, @decidable_eq_of_prod_left B S ⟨s⟩ (hob s a t h))) hS)
 
+section is_well_formed
+
+@[class]
+inductive is_well_formed : ∀ {A B C : Type}, oracle_comp A B C → Prop
+| well_formed_oc_query {A B : Type} (a : A) : 
+    is_well_formed (oc_query a : oracle_comp A B B)
+| well_formed_oc_ret {A B C : Type} (c : comp C) (hc : c.is_well_formed) :
+    is_well_formed (oc_ret c : oracle_comp A B C)
+| well_formed_oc_bind {A B C D : Type} (oc : oracle_comp A B C) (od : C → oracle_comp A B D)
+    (hoc : is_well_formed oc) (hod : ∀ c, is_well_formed $ od c) :
+    is_well_formed (oc_bind oc od)
+| well_formed_oc_run {A B C A' B' S : Type} [decidable_eq A] [decidable_eq B] [decidable_eq S]
+    (oc : oracle_comp A B C) (ob : S → A → oracle_comp A' B' (B × S)) (s : S)
+    (hoc : is_well_formed oc) (hob : ∀ s a, is_well_formed $ ob s a) :
+    is_well_formed (oc_run oc ob s)
+
+@[simp]
+lemma oc_query_is_well_formed {A B : Type} (a : A) :
+  (oc_query a : oracle_comp A B B).is_well_formed :=
+is_well_formed.well_formed_oc_query a
+
+instance oc_query.is_well_formed {A B : Type} (a : A) :
+  (oc_query a : oracle_comp A B B).is_well_formed :=
+by simp
+
+@[simp]
+lemma oc_ret_is_well_formed_iff {A B C : Type} (c : comp C) :
+  (oc_ret c : oracle_comp A B C).is_well_formed ↔ c.is_well_formed :=
+begin
+  refine ⟨λ h, _, λ h, is_well_formed.well_formed_oc_ret c h⟩,
+  cases h,
+  exact h_hc,
+end
+
+instance oc_ret.is_well_formed {A B C : Type} (c : comp C)
+  [c.is_well_formed] : (oc_ret c : oracle_comp A B C).is_well_formed :=
+by simpa
+
+@[simp]
+lemma oc_bind_is_well_formed_iff {A B C D : Type} 
+  (oc : oracle_comp A B C) (od : C → oracle_comp A B D) :
+  (oc_bind oc od).is_well_formed ↔ 
+    oc.is_well_formed ∧ ∀ c, (od c).is_well_formed :=
+begin
+  sorry,
+end
+
+end is_well_formed
+
 /-- Evaluation distribution of an `oracle_comp A B C` as a `comp A`.
 `S` is the type of the internal state of the `A` to `B` oracle, and `s` is the initial state.
-`f` takes the current oracle state and an `A` value, and computes a `B` value and new oracle state. -/
+`o` takes the current oracle state and an `A` value, and computes a `B` value and new oracle state. -/
 def eval_distribution (oc : oracle_comp A B C) :
-  Π (S : Type) [decidable_eq S] (f : S → A → comp (B × S)) (s : S), comp (C × S) :=
+  Π {S : Type} [decidable_eq S] (s : S) (o : S → A → comp (B × S)), comp (C × S) :=
 begin
   induction oc with A B a A B C c A B C D oc od hoc hod A B C A' B' S' hA hB hS' oc ob s' hoc hob,
-  { exact λ S hS o s, o s a },
-  { intros S hS o s,
-    haveI : decidable_eq C := comp.decidable_eq_of_comp c,
-    refine c.bind (λ c, comp.ret (c, s)) },
-  { introsI S hS o s,
-    exact (hoc S o s).bind (λ cs', hod cs'.fst S o cs'.snd) },
-  { introsI S hS o' s,
-    specialize hoc (S' × S) (λ ss a, (hob ss.fst a S o' ss.snd).bind 
-      (λ x, comp.ret (x.1.1, (x.1.2, x.2)))) (s', s),
+  { exact λ S hS s o, o s a },
+  { exact λ S hS s o,
+      c.bind (λ x, @comp.ret (C × S) (@prod.decidable_eq C S (comp.decidable_eq_of_comp c) hS) (x, s)) },
+  { exact λ S hS s o, (@hoc S hS s o).bind (λ cs', @hod cs'.fst S hS cs'.snd o) },
+  { introsI S hS s o',
+    specialize hoc (s', s) (λ ss a, (hob ss.fst a ss.snd o').bind 
+      (λ x, comp.ret (x.1.1, (x.1.2, x.2)))) ,
     haveI : decidable_eq (C × S' × S) := comp.decidable_eq_of_comp hoc,
     haveI : inhabited (S' × S) := ⟨(s', s)⟩,
     haveI : decidable_eq C := decidable_eq_of_prod_left C (S' × S),
     refine (hoc.bind $ λ x, comp.ret ((x.1, x.2.1), x.2.2)) }
+end
+
+@[simp]
+lemma eval_distribution_oc_query {A B S : Type} [decidable_eq S]
+  (a : A) (s : S) (o : S → A → comp (B × S)) :
+  (oc_query a : oracle_comp A B B).eval_distribution s o = o s a := 
+rfl
+
+@[simp]
+lemma eval_distribution_oc_ret {A B C S : Type} [hS : decidable_eq S]
+  (c : comp C) (s : S) (o : S → A → comp (B × S)) :
+  (oc_ret c : oracle_comp A B C).eval_distribution s o =
+    c.bind (λ x, @comp.ret (C × S) (@prod.decidable_eq C S (comp.decidable_eq_of_comp c) hS) (x, s)) :=
+rfl 
+
+@[simp]
+lemma eval_distribution_oc_bind {A B C D S : Type} [hS : decidable_eq S]
+  (oc : oracle_comp A B C) (od : C → oracle_comp A B D)
+  (s : S) (o : S → A → comp (B × S)) :
+  (oc_bind oc od).eval_distribution s o = 
+    (oc.eval_distribution s o).bind (λ cs', (od cs'.1).eval_distribution cs'.2 o) :=
+rfl
+
+@[simp]
+instance eval_distribution_well_formed {S : Type} [decidable_eq S] 
+  (oc : oracle_comp A B C) [hoc : oc.is_well_formed] :
+  ∀ (s : S) (o : S → A → comp (B × S)) (ho : ∀ s a, (o s a).is_well_formed),
+    (oc.eval_distribution s o).is_well_formed :=
+begin
+  unfreezingI { induction oc with A B a A B C c A B C D oc od hoc' hod A B C A' B' S' hA hB hS' oc ob s' hoc hob generalizing },
+  {
+    intros s o ho,
+    simpa only using ho s a,
+  },
+  {
+    intros s o ho,
+    simp,
+    exact (oc_ret_is_well_formed_iff c).1 hoc,
+  },
+  {
+    intros s o ho,
+    simp,
+    rw oc_bind_is_well_formed_iff at hoc,
+    haveI : oc.is_well_formed := hoc.1,
+    refine ⟨hoc' s o ho, λ c s' h, _⟩,
+    haveI : (od c).is_well_formed := hoc.2 c,
+    exact hod c s' o ho,
+  },
+  {
+    sorry,
+  }
 end
 
 /-- Evaluation distribution for a stateless oracle with `f` simulating the oracle. -/
@@ -76,16 +174,15 @@ def stateless_eval_distribution [decidable_eq B] [decidable_eq C]
 begin
   let f' : unit → A → comp (B × unit) :=
     λ _ a, comp.bind (f a) (λ b, comp.ret (b, ())),
-  refine (oc.eval_distribution unit f' ()).bind (λ c, comp.ret c.1),
+  refine (oc.eval_distribution () f').bind (λ c, comp.ret c.1),
 end
 
 @[simp]
 instance stateless_eval_distribution_well_formed [decidable_eq B] [decidable_eq C]
-  (oc : oracle_comp A B C) (f : A → comp B) :
-  (oc.stateless_eval_distribution f).is_well_formed :=
-begin
-  sorry,
-end
+  (oc : oracle_comp A B C) [hoc : oc.is_well_formed]
+  (o : A → comp B) [ho : ∀ a, (o a).is_well_formed] :
+  (oc.stateless_eval_distribution o).is_well_formed :=
+by simp [stateless_eval_distribution]
 
 
 end oracle_comp
